WIP

bedrock2/src/bedrock2Examples/roughtime.v
@@ -28,6 +28,8 @@ Proof.
   intros s.
 Admitted.
 
+Opaque Z_of_string.
+
 Definition createTimestampMessage :=
   let buffer := "buffer" in
   let i := "i" in
@@ -56,8 +58,8 @@ Definition createTimestampMessage :=
     store4(buffer + coq:(120), coq:(Z_of_string "MIDP"));
     store4(buffer + coq:(124), coq:(Z_of_string "ROOT"));
     
-    store4(buffer + coq:(128), coq:(Ox"4242"));
-    store4(buffer + coq:(132), coq:(Ox"42424242"));
+    store4(buffer + coq:(128), coq:(Ox"42"));
+    store4(buffer + coq:(132), coq:(Ox"4242"));
     i = (coq:(64)); while (i) { i = (i - coq:(4));
       store4(buffer + coq:(200) - i, coq:(Ox"42"))
     };
@@ -80,9 +82,7 @@ Definition createTimestampMessage :=
  
     i = (coq:(48)); while (i) { i = (i - coq:(4));
       store4(buffer + coq:(352) - i, coq:(Ox"42"))
-    };
-
-    store4(buffer + coq:(356), coq:(Ox"43"))))).
+    }))).
     
 Require Import bedrock2.ToCString.
    Definition allProgsAsCString : string :=
@@ -109,25 +109,30 @@ Section WithParameters.
   Infix "*" := (sep).
   Infix "*" := (sep) : type_scope.
 
-  Infix "+" := (word.add).
-  Infix "+" := (word.add) : type_scope.
+  Local Infix "^+" := word.add  (at level 50, left associativity).
+  Local Infix "^-" := word.sub  (at level 50, left associativity).
+  Local Infix "^*" := word.mul  (at level 50, left associativity).
+  Local Notation "/_" := word.of_Z.      (* smaller angle: squeeze a Z into a word *)
+  Local Notation "\_" := word.unsigned.  (* supposed to be a denotation bracket;
+                                          or bigger angle: let a word fly into the large Z space *)
+  
 
   Notation array32 := (array scalar32 (word.of_Z 4)).
   
   Definition stringToWord (s : string) := word.of_Z (Z_of_string s).
 
   Definition size_field (addr: Semantics.word) (entries : list entry) : mem -> Prop :=
-    scalar32 addr (word.of_Z (Z.of_nat (List.length entries))).
+    scalar32 addr (/_ (Z.of_nat (List.length entries))).
   
   Definition offsets_field (addr: Semantics.word) (entries : list entry) : mem -> Prop :=
-    array32 (addr + (word.of_Z 4)) 
+    array32 (addr ^+ (word.of_Z 4)) 
             (List.map (fun entry => (snd (fst entry))) (tl entries)).
   
   Definition tags_offset (entries : list entry) :=
     (4 + 4 * (List.length (tl entries)))%nat.
   
   Definition tags_field (addr: Semantics.word) (entries : list entry) : mem -> Prop :=
-    array32 (addr + (word.of_Z (Z.of_nat (tags_offset entries))))
+    array32 (addr ^+ (word.of_Z (Z.of_nat (tags_offset entries))))
             (List.map (fun entry => stringToWord (fst (fst entry))) entries).
 
   Definition contents_offset (entries : list entry) :=
@@ -135,43 +140,44 @@ Section WithParameters.
   
   Definition message_ok (addr: Semantics.word) (entries : list entry): mem -> Prop :=
     size_field addr entries * offsets_field addr entries * tags_field addr entries *
-    let current_addr := addr + (word.of_Z (Z.of_nat (contents_offset entries))) in
-    List.fold_left (fun P entry => (snd entry) (current_addr + (snd (fst entry))) * P)
+    let current_addr := addr ^+ (word.of_Z (Z.of_nat (contents_offset entries))) in
+    List.fold_left (fun P entry => (snd entry) (current_addr ^+ (snd (fst entry))) * P)
                    entries (emp True).
   
-  Definition repeat_dummy n := fun addr => array32 (addr: Semantics.word) (List.repeat (word.of_Z (Ox"42")) n).
+  Definition repeat_dummy n := fun addr => array32 (addr: Semantics.word) (List.repeat (/_ (Ox"4242")) n).
+
 
   Definition srep_val : list entry :=
-    [("RADI", word.of_Z 0, fun _ => (emp True));
-    ("MIDP", word.of_Z 4,  fun _ => (emp True));
-    ("ROOT", word.of_Z 12,  fun _ => (emp True))
+    [("RADI", word.of_Z 0, repeat_dummy 1);
+    ("MIDP", word.of_Z 4,  repeat_dummy 2);
+    ("ROOT", word.of_Z 12, repeat_dummy 64)
     ].
 
   Definition dele_val : list entry :=
-    [("MINT", word.of_Z 0, fun _ => (emp True));
-    ("MAXT", word.of_Z 32,  fun _ => (emp True));
-    ("PUBK", word.of_Z 40,  fun _ => (emp True))
+    [("MINT", word.of_Z 0, repeat_dummy 8);
+    ("MAXT", word.of_Z 32, repeat_dummy 8);
+    ("PUBK", word.of_Z 40, repeat_dummy 64)
     ].
 
   Definition cert_val : list entry :=
-    [("SIG", word.of_Z 0, fun _ => (emp True));
+    [("SIG", word.of_Z 0, repeat_dummy 64);
     ("DELE", word.of_Z 64, fun addr => message_ok addr dele_val)
     ].
   
   
   Definition message_val : list entry :=
-    [("SIG", word.of_Z 0, fun _ => (emp True));
+    [("SIG", word.of_Z 0, fun addr => (array32 addr (List.repeat (/_ (Ox"42")) 64)));
     ("PATH", word.of_Z 64, fun _ => (emp True));
     ("SREP", word.of_Z 64, fun addr => message_ok addr srep_val);
     ("CERT", word.of_Z 164, fun addr => message_ok addr cert_val);
-    ("INDX", word.of_Z 316, fun _ => (emp True))
+    ("INDX", word.of_Z 316, fun addr => (array32 addr (List.repeat (/_ (Ox"42")) 64)))
     ].
     
 
   Instance spec_of_createTimestampMessage : spec_of "createTimestampMessage" := fun functions =>
     forall p_addr buf R m t,
       ((array32 p_addr buf) * R) m ->
-      List.length buf = 1024%nat ->
+      List.length buf = 352%nat ->
       WeakestPrecondition.call functions "createTimestampMessage" t m [p_addr]
       (fun t' m' rets => t = t' /\ rets = nil /\ (message_ok p_addr message_val * R) m'). 
   
@@ -183,31 +189,30 @@ Section WithParameters.
    Ltac subst_words :=
      repeat match goal with x := _ : word.rep |- _ => subst x end.
    
-   Notation "a |-> v" := (scalar32 a (word.of_Z v)) (at level 30).
-   Notation lit := (@word.of_Z (@width (@semantics_parameters p))
-                               (@Semantics.word (@semantics_parameters p))).
+   Notation "a |-> v" := (scalar32 a (/_ v)) (at level 30).
+   Notation "l [[ n  |:= v ]]" := (List.listUpdate l n v) (left associativity, at level 50).
 
    Ltac word_simplify :=
        match goal with
-       | |- context [?a + ?b] => progress (ring_simplify (a + b))
-       | |- context [word.sub ?a ?b] => progress (ring_simplify (word.sub a b))
+       | |- context [?a ^+ ?b] => progress (ring_simplify (a ^+ b))
+       | |- context [?a ^- ?b] => progress (ring_simplify (a ^- b))
        end.
 
    Ltac word_Z_unsigned :=
      match goal with
-     | |- context [ (word.unsigned (word.of_Z ?z))] => rewrite (word.unsigned_of_Z z); change (word.wrap z) with z
-     | |- context [word.of_Z (word.unsigned ?z)] => rewrite (word.of_Z_unsigned z)
+     | |- context [\_ (/_ ?z)] => rewrite (word.unsigned_of_Z z); change (word.wrap z) with z
+     | |- context [/_ (\_ ?z)] => rewrite (word.of_Z_unsigned z)
      end.
 
    Ltac word_simplify_in H :=
        match type of H with 
-       | context [?a + ?b] => progress (ring_simplify (a + b) in H)
-       | context [word.sub ?a ?b] => progress (ring_simplify (word.sub a b) in H)
+       | context [?a ^+ ?b] => progress (ring_simplify (a ^+ b) in H)
+       | context [?a ^- ?b] => progress (ring_simplify (a ^- b) in H)
        end.
    Ltac word_Z_unsigned_in H:=
      match type of H with
-     | context [word.unsigned (word.of_Z ?z)] => rewrite (word.unsigned_of_Z z) in H; change (word.wrap z) with z in H
-     | context [word.of_Z (word.unsigned ?z)] => rewrite (word.of_Z_unsigned z) in H
+     | context [\_ (/_ ?z)] => rewrite (word.unsigned_of_Z z) in H; change (word.wrap z) with z in H
+     | context [/_ (\_ ?z)] => rewrite (word.of_Z_unsigned z) in H
      end.
 
    Ltac word_unwrap t :=
@@ -217,12 +222,764 @@ Section WithParameters.
      unfold word.wrap in H; rewrite (Zmod_small t) in H; [| assert (0 <= t < 2^width) by blia; assumption].
 
    Definition todo : False. Admitted.
+
+   Ltac subst_nat :=
+     match goal with
+     | H : @eq nat ?x ?y |- context[?x] => rewrite H
+     end.
+(*
+   Ltac array_straightline :=
+     match goal with
+     | x : ?p ?m |- @WeakestPrecondition.store _ Syntax.access_size.four ?m ?addr' ?v _ => match p with context [array32 ?addr ?xs] =>
+       remember (Z.to_nat ((\_ (addr' ^- addr)) / 4)) as n eqn:Heqn;
+       ring_simplify (addr' ^- addr) in Heqn;
+       word_Z_unsigned_in Heqn;
+       cbv in Heqn; (*Dangerous*)
+       assert (List.length (xs [[n |:= v]]) = 1024%nat) by (rewrite List.listUpdate_length; blia);
+       eapply (array_store_four_of_sep_32bit _ addr addr' n xs _ (word.of_Z 4)); subst ;[try word_Z_unsigned; try ring | ecancel_assumption | subst_nat; blia |]
+ end
+     end.
+
+   Ltac array_first_cleanup H :=
+     rewrite List.skipn_skipn in H;
+  *)   
+   
+   Ltac skipn_simpl :=
+     match goal with
+     | H : context [List.skipn ?a (List.skipn ?b ?l)] |- _ =>
+       rewrite List.skipn_skipn in H;
+         cbn[Nat.add] in H
+     end.
+
+   
+   Ltac array_first_straightline :=
+     match goal with
+     | H : ?p ?m |- @WeakestPrecondition.store _ access_size.four ?m ?addr' _ _ =>
+       match p with
+         context [array32 ?addr ?xs] =>
+         subst_words;
+         try (rewrite List.skipn_skipn in H; cbn[Nat.add] in H);
+         array_app_cons_sep;
+         try word_simplify_in H;
+         eapply array_first_store_four_of_sep_32bit;
+         [ reflexivity | ecancel_assumption | try rewrite skipn_length; blia |];
+         repeat straightline
+       end
+     end.
+
+   Ltac array_first_before :=
+     match goal with
+     | H : ?p ?m |- @WeakestPrecondition.store _ access_size.four ?m ?addr' _ _ =>
+       subst_words;
+       eapply array_first_store_four_of_sep_32bit;
+       [ reflexivity | ecancel_assumption | try rewrite skipn_length; blia |];
+       array_app_cons_sep;
+       repeat straightline
+     end.
+   
+   Ltac array_first_after :=
+     match goal with
+     | H : context [array32 (word.add ?a ?b) (List.skipn ?m ?l)] |- _ =>
+       ring_simplify (word.add a b) in H;
+       try (rewrite List.skipn_skipn in H; cbn[Nat.add] in H)
+     end.
+   
+   Ltac array_first_straightline' := array_first_before; array_first_after.
+
+   Ltac subst_skipn :=
+     match goal with
+     | H : context [List.skipn ?n ?buf] |- _ =>
+       match goal with
+       | H' : List.length ?buf = ?l |- _ =>
+         is_var buf;
+         let buf' := fresh buf in
+         let H0 := fresh H in
+         let H1 := fresh H in
+         remember (List.skipn n buf) as buf' eqn:H0;
+         pose proof (H1 := f_equal (@List.length _) H0);
+         rewrite skipn_length, H' in H1;
+         cbn[Nat.sub] in H1;
+         clear H' H0 buf;
+         rename buf' into buf
+       end
+     end.
+
+   Ltac array_straightline :=
+     match goal with
+     | x : ?p ?m |- @WeakestPrecondition.store _ Syntax.access_size.four ?m ?addr' ?v _ =>
+       match p with
+       | context [array32 ?addr ?xs] =>
+         eapply (array_store_four_of_sep' _ addr addr' xs);
+         [ecancel_assumption |];
+         ring_simplify (addr' ^- addr);
+         word_Z_unsigned;
+         progress cbv zeta;
+         split; [try reflexivity | split; [simpl (Z.to_nat _); try blia|] ]
+       end
+     end.
+   
+   (*Ideally I want to do context on two terms inside one hypothesis*)
    
    Lemma createTimestampMessage_ok : program_logic_goal_for_function! createTimestampMessage.
    Proof.
      repeat straightline.
-     do 10 (destruct buf; [inversion H0|]).
-     inversion H0; clear H0.
+     eapply (array_store_four_of_sep' _); [ecancel_assumption|].
+     
+     ring_simplify (p_addr ^- p_addr).
+     word_Z_unsigned.
+     ring_simplify (0 / 4).
+     match goal with
+     | |- context [Z.to_nat (?a / 4)] =>
+       let r := isZcst a in
+       lazymatch r with | true =>
+         let x := eval cbv in (Z.to_nat (a/4)) in change (Z.to_nat (a/4)) with x
+       end;
+       idtac a r
+     end.
+     simpl (Z.to_nat _).
+     rewrite 
+     
+     Search word.of_Z word.unsigned.
+     
+     
+     word_Z_unsigned.
+     cbv zeta.
+     word_Z_unsigned.
+     split; [reflexivity|].
+     
+     split.
+     match goal with
+     | x : ?p ?m |- @WeakestPrecondition.store _ Syntax.access_size.four ?m ?addr' ?v _ =>
+       match p with
+       | context [array32 ?addr ?xs] =>
+         eapply (array_store_four_of_sep' _ addr addr' xs);
+         [ecancel_assumption |];
+         ring_simplify (addr' ^- addr);
+         cbv zeta
+       end
+     end.
+
+     array_straightline.
+     eapply (array_store_four_of_sep' _ _ _ _); [ecancel_assumption|].
+     ring_simplify term+
+     cbv zeta.
+     
+     
+     array_straightline.
+     array_straightline; ring_simplify (p_addr ^- p_addr).
+     
+     array_straightline.
+     { ring_simplify (p_addr ^- p_addr). word_Z_unsigned. reflexivity. }
+     { admit. }
+     cbv zeta.
+                         
+     eapply array_store_four_of_sep'; [reflexivity| ecancel_assumption| |].
+     { word_simplify. word_Z_unsigned. 
+     
+     
+     
+     assert (Datatypes.length buf = 352%nat) by blia; clear H0.
+     do 10 array_first_straightline'.
+     clear H9 H8 H7 H6 H5 H4 H3 H2 H0 H.
+     subst_skipn.
+     remember ((p_addr ^+ /_ 36) |-> Z_of_string "INDX" *
+         ((p_addr ^+ /_ 32) |-> Z_of_string "CERT" *
+          ((p_addr ^+ /_ 28) |-> Z_of_string "SREP" *
+           ((p_addr ^+ /_ 24) |-> Z_of_string "PATH" *
+            ((p_addr ^+ /_ 20) |-> Z_of_string "SIG" *
+             ((p_addr ^+ /_ 16) |-> 316 *
+              ((p_addr ^+ /_ 12) |-> 164 *
+               ((p_addr ^+ /_ 8) |-> 64 * ((p_addr ^+ /_ 4) |-> 64 * (p_addr |-> 5 * R)))))))))%type) as P.
+     assert ((P * array32 (p_addr ^+ /_ 40) buf) m9) by (rewrite HeqP; ecancel_assumption).
+     clear H10.
+     subst i.     
+
+     refine ((TailRecursion.tailrec (HList.polymorphic_list.cons _ HList.polymorphic_list.nil) ("i"::"buffer"::nil)%list%string (fun V R T M I BUFFER => PrimitivePair.pair.mk (exists i, V = 64 - 4 * (Z.of_nat i) /\ V = word.unsigned I /\ BUFFER = p_addr /\ (array32 (p_addr ^+ (/_ 40)) (List.repeat (word.of_Z (Ox"42")) i) * array32 (p_addr ^+ (/_ (104 - V))) (List.skipn i buf) * P * R) M) (fun t m i buff => t = T /\ buff = p_addr /\ (P * array32 (p_addr ^+ /_ 40) (List.repeat (word.of_Z (Ox"42")) 16) * array32 (p_addr ^+ (/_ (104))) (List.skipn 16%nat buf) * R) m))) _ _ _ _ _ _ _);
+      cbn [reconstruct map.putmany_of_list HList.tuple.to_list
+           HList.hlist.foralls HList.tuple.foralls
+           HList.hlist.existss HList.tuple.existss
+           HList.hlist.apply  HList.tuple.apply
+           HList.hlist
+
+           (* List.repeat *) Datatypes.length
+           HList.polymorphic_list.repeat HList.polymorphic_list.length
+           PrimitivePair.pair._1 PrimitivePair.pair._2] in *.
+     { repeat straightline. }
+     { eapply (Z.lt_wf 0). }
+     { exists 0%nat.
+       split; [auto| split; [word_Z_unsigned; blia| split; [auto|] ] ] .
+       simpl (104 - _).
+       cbn [List.repeat Array.array List.skipn List.map].
+       ecancel_assumption. }
+     { repeat straightline.
+       2: {
+         split; try split; auto.
+         replace x2 with 16%nat in H0, H4 by blia.
+         simpl in H0.
+         rewrite H0 in *.
+         simpl (104-0) in H4.
+         ecancel_assumption. }
+       
+       subst_words.
+       word_simplify.
+       subst v.
+       repeat word_simplify_in H4.
+       word_Z_unsigned_in H4.
+       pose proof (word.unsigned_range x0).
+       assert (List.length (List.skipn x2 buf) <> 0%nat) by (rewrite List.skipn_length; blia).
+       destruct (List.skipn x2 buf) eqn:H17; try contradiction.
+       array_app_cons_sep.
+       repeat straightline.
+       subst_words.
+       eexists; eexists; split.
+       { exists (1 + x2)%nat.
+         replace (64 - 4 * Z.of_nat (1 + x2)) with (60 - 4 * Z.of_nat x2) by blia.
+         split; auto.
+         split; [|split; [auto|] ].
+         { rewrite word.unsigned_sub.
+           word_Z_unsigned.
+           word_unwrap (word.unsigned x0 - 4).
+           blia.
+         }
+         { pose proof (f_equal word.of_Z H0).
+           word_Z_unsigned_in H8.
+           rewrite H8 in H7.
+           cbn[Nat.add List.repeat].
+           rewrite repeat_cons.
+           array_app_cons_sep.
+           rewrite repeat_length, <- List.tl_skipn, H17.
+           cbn[List.tl].
+           repeat word_simplify.
+           repeat word_simplify_in H7.
+           change (66) with (Ox "42") in H7.
+           ecancel_assumption. }
+       }
+       split; [blia| auto].
+     }
+     repeat straightline.
+     clear H.
+     do 8 array_first_straightline'.
+     clear H7 H6 H5 H4 H3 H1 H0 H.
+     repeat straightline.
+     subst i.
+     subst_skipn.
+
+     remember ((p_addr ^+ /_ 132) |-> 16962 *
+        ((p_addr ^+ /_ 128) |-> 66 *
+         ((p_addr ^+ /_ 124) |-> Z_of_string "ROOT" *
+          ((p_addr ^+ /_ 120) |-> Z_of_string "MIDP" *
+           ((p_addr ^+ /_ 116) |-> Z_of_string "RADI" *
+            ((p_addr ^+ /_ 112) |-> 12 *
+             ((p_addr ^+ /_ 108) |-> 4 *
+              ((p_addr ^+ /_ 104) |-> 3 *
+               (P * array32 (p_addr ^+ /_ 40) (repeat (/_ (Ox "42")) 16)))))))))%type) as Q.
+     assert ((Q * array32 (p_addr ^+ /_ 136) buf) m7) by (rewrite HeqQ; ecancel_assumption).
+     clear H8.
+
+     refine ((TailRecursion.tailrec (HList.polymorphic_list.cons _ HList.polymorphic_list.nil) ("i"::"buffer"::nil)%list%string (fun V R T M I BUFFER => PrimitivePair.pair.mk (exists i, V = 64 - 4 * (Z.of_nat i) /\ V = word.unsigned I /\ BUFFER = p_addr /\ (array32 (p_addr ^+ (/_ 136)) (List.repeat (word.of_Z (Ox"42")) i) * array32 (p_addr ^+ (/_ (200 - V))) (List.skipn i buf) * Q * R) M) (fun t m i buff => t = T /\ buff = p_addr /\ (Q * array32 (p_addr ^+ /_ 136) (List.repeat (word.of_Z (Ox"42")) 16) * array32 (p_addr ^+ (/_ (200))) (List.skipn 16%nat buf) * R) m))) _ _ _ _ _ _ _);
+      cbn [reconstruct map.putmany_of_list HList.tuple.to_list
+           HList.hlist.foralls HList.tuple.foralls
+           HList.hlist.existss HList.tuple.existss
+           HList.hlist.apply  HList.tuple.apply
+           HList.hlist
+
+           (* List.repeat *) Datatypes.length
+           HList.polymorphic_list.repeat HList.polymorphic_list.length
+           PrimitivePair.pair._1 PrimitivePair.pair._2] in *.
+     { repeat straightline. }
+     { eapply (Z.lt_wf 0). }
+     { exists 0%nat.
+       split; [auto| split; [word_Z_unsigned; blia| split; [auto|] ] ] .
+       simpl (200 - _).
+       cbn [List.repeat Array.array List.skipn List.map].
+       ecancel_assumption. }
+     { repeat straightline.
+       2: {
+         split; try split; auto.
+         replace x3 with 16%nat in H0, H4 by blia.
+         simpl in H0.
+         rewrite H0 in *.
+         simpl (200-0) in H4.
+         ecancel_assumption. }
+       
+       subst_words.
+       word_simplify.
+       subst v.
+       repeat word_simplify_in H4.
+       word_Z_unsigned_in H4.
+       pose proof (word.unsigned_range x1).
+       assert (List.length (List.skipn x3 buf) <> 0%nat) by (rewrite List.skipn_length; blia).
+       destruct (List.skipn x3 buf) eqn:H17; try contradiction.
+       array_app_cons_sep.
+       repeat straightline.
+       subst_words.
+       eexists; eexists; split.
+       { exists (1 + x3)%nat.
+         replace (64 - 4 * Z.of_nat (1 + x3)) with (60 - 4 * Z.of_nat x3) by blia.
+         split; auto.
+         split; [|split; [auto|] ].
+         { rewrite word.unsigned_sub.
+           word_Z_unsigned.
+           word_unwrap (word.unsigned x1 - 4).
+           blia.
+         }
+         { pose proof (f_equal word.of_Z H0).
+           word_Z_unsigned_in H8.
+           rewrite H8 in H7.
+           cbn[Nat.add List.repeat].
+           rewrite repeat_cons.
+           array_app_cons_sep.
+           rewrite repeat_length, <- List.tl_skipn, H17.
+           cbn[List.tl].
+           repeat word_simplify.
+           repeat word_simplify_in H7.
+           change (66) with (Ox "42") in H7.
+           ecancel_assumption. }
+       }
+       split; [blia| auto].
+     }
+     repeat straightline.
+     clear H.
+     do 4 array_first_straightline'.
+     clear H3 H2 H0 H.
+     repeat straightline.
+     subst i.
+     subst_skipn.
+
+     remember ((p_addr ^+ /_ 212) |-> Z_of_string "DELE" *
+        ((p_addr ^+ /_ 208) |-> Z_of_string "SIG" *
+         ((p_addr ^+ /_ 204) |-> 64 *
+          ((p_addr ^+ /_ 200) |-> 2 *
+           (Q * array32 (p_addr ^+ /_ 136) (repeat (/_ (Ox "42")) 16)))))) as P1.
+     assert ((P1 * array32 (p_addr ^+ /_ 216) buf) m3) by (rewrite HeqP1; ecancel_assumption).
+     clear H4.
+
+     refine ((TailRecursion.tailrec (HList.polymorphic_list.cons _ HList.polymorphic_list.nil) ("i"::"buffer"::nil)%list%string (fun V R T M I BUFFER => PrimitivePair.pair.mk (exists i, V = 64 - 4 * (Z.of_nat i) /\ V = word.unsigned I /\ BUFFER = p_addr /\ (array32 (p_addr ^+ (/_ 216)) (List.repeat (word.of_Z (Ox"42")) i) * array32 (p_addr ^+ (/_ (280 - V))) (List.skipn i buf) * P1 * R) M) (fun t m i buff => t = T /\ buff = p_addr /\ (P1 * array32 (p_addr ^+ /_ 216) (List.repeat (word.of_Z (Ox"42")) 16) * array32 (p_addr ^+ (/_ (280))) (List.skipn 16%nat buf) * R) m))) _ _ _ _ _ _ _);
+      cbn [reconstruct map.putmany_of_list HList.tuple.to_list
+           HList.hlist.foralls HList.tuple.foralls
+           HList.hlist.existss HList.tuple.existss
+           HList.hlist.apply  HList.tuple.apply
+           HList.hlist
+
+           (* List.repeat *) Datatypes.length
+           HList.polymorphic_list.repeat HList.polymorphic_list.length
+           PrimitivePair.pair._1 PrimitivePair.pair._2] in *.
+     { repeat straightline. }
+     { eapply (Z.lt_wf 0). }
+     { exists 0%nat.
+       split; [auto| split; [word_Z_unsigned; blia| split; [auto|] ] ] .
+       simpl (280 - _).
+       cbn [List.repeat Array.array List.skipn List.map].
+       ecancel_assumption. }
+     { repeat straightline.
+       2: {
+         split; try split; auto.
+         replace x4 with 16%nat in H0, H4 by blia.
+         simpl in H0.
+         rewrite H0 in *.
+         simpl (280-0) in H4.
+         ecancel_assumption. }
+       
+       subst_words.
+       word_simplify.
+       subst v.
+       repeat word_simplify_in H4.
+       word_Z_unsigned_in H4.
+       pose proof (word.unsigned_range x2).
+       assert (List.length (List.skipn x4 buf) <> 0%nat) by (rewrite List.skipn_length; blia).
+       destruct (List.skipn x4 buf) eqn:H17; try contradiction.
+       array_app_cons_sep.
+       repeat straightline.
+       subst_words.
+       eexists; eexists; split.
+       { exists (1 + x4)%nat.
+         replace (64 - 4 * Z.of_nat (1 + x4)) with (60 - 4 * Z.of_nat x4) by blia.
+         split; auto.
+         split; [|split; [auto|] ].
+         { rewrite word.unsigned_sub.
+           word_Z_unsigned.
+           word_unwrap (word.unsigned x2 - 4).
+           blia.
+         }
+         { pose proof (f_equal word.of_Z H0).
+           word_Z_unsigned_in H8.
+           rewrite H8 in H7.
+           cbn[Nat.add List.repeat].
+           rewrite repeat_cons.
+           array_app_cons_sep.
+           rewrite repeat_length, <- List.tl_skipn, H17.
+           cbn[List.tl].
+           repeat word_simplify.
+           repeat word_simplify_in H7.
+           change (66) with (Ox "42") in H7.
+           ecancel_assumption. }
+       }
+       split; [blia| auto].
+     }
+     repeat straightline.
+     clear H.
+     do 6 array_first_straightline'.
+     clear H5 H4 H3 H1 H0 H.
+     repeat straightline.
+     subst i.
+     subst_skipn.
+
+     remember ((p_addr ^+ /_ 300) |-> Z_of_string "MAXT" *
+        ((p_addr ^+ /_ 296) |-> Z_of_string "MINT" *
+         ((p_addr ^+ /_ 292) |-> Z_of_string "PUBK" *
+          ((p_addr ^+ /_ 288) |-> 40 *
+           ((p_addr ^+ /_ 284) |-> 32 *
+            ((p_addr ^+ /_ 280) |-> 3 *
+             (P1 * array32 (p_addr ^+ /_ 216) (repeat (/_ (Ox "42")) 16)))))))%type) as P2.
+     assert ((P2 * array32 (p_addr ^+ /_ 304) buf) m5) by (rewrite HeqP2; ecancel_assumption).
+     clear H6.
+     
+     refine ((TailRecursion.tailrec (HList.polymorphic_list.cons _ HList.polymorphic_list.nil) ("i"::"buffer"::nil)%list%string (fun V R T M I BUFFER => PrimitivePair.pair.mk (exists i, V = 48 - 4 * (Z.of_nat i) /\ V = word.unsigned I /\ BUFFER = p_addr /\ (array32 (p_addr ^+ (/_ 304)) (List.repeat (word.of_Z (Ox"42")) i) * array32 (p_addr ^+ (/_ (352 - V))) (List.skipn i buf) * P2 * R) M) (fun t m i buff => t = T /\ buff = p_addr /\ (P2 * array32 (p_addr ^+ /_ 304) (List.repeat (word.of_Z (Ox"42")) 12) * array32 (p_addr ^+ (/_ (352))) (List.skipn 12%nat buf) * R) m))) _ _ _ _ _ _ _);
+      cbn [reconstruct map.putmany_of_list HList.tuple.to_list
+           HList.hlist.foralls HList.tuple.foralls
+           HList.hlist.existss HList.tuple.existss
+           HList.hlist.apply  HList.tuple.apply
+           HList.hlist
+
+           (* List.repeat *) Datatypes.length
+           HList.polymorphic_list.repeat HList.polymorphic_list.length
+           PrimitivePair.pair._1 PrimitivePair.pair._2] in *.
+     { repeat straightline. }
+     { eapply (Z.lt_wf 0). }
+     { exists 0%nat.
+       split; [auto| split; [word_Z_unsigned; blia| split; [auto|] ] ] .
+       simpl (352 - _).
+       cbn [List.repeat Array.array List.skipn List.map].
+       ecancel_assumption. }
+     { repeat straightline.
+       2: {
+         split; try split; auto.
+         replace x5 with 12%nat in H0, H4 by blia.
+         simpl in H0.
+         rewrite H0 in *.
+         simpl (352-0) in H4.
+         ecancel_assumption. }
+       
+       subst_words.
+       word_simplify.
+       subst v.
+       repeat word_simplify_in H4.
+       word_Z_unsigned_in H4.
+       pose proof (word.unsigned_range x3).
+       assert (List.length (List.skipn x5 buf) <> 0%nat) by (rewrite List.skipn_length; blia).
+       destruct (List.skipn x5 buf) eqn:H17; try contradiction.
+       array_app_cons_sep.
+       repeat straightline.
+       subst_words.
+       eexists; eexists; split.
+       { exists (1 + x5)%nat.
+         split; auto.
+         split; [|split; [auto|] ].
+         { rewrite word.unsigned_sub.
+           word_Z_unsigned.
+           word_unwrap (word.unsigned x3 - 4).
+           blia.
+         }
+         { pose proof (f_equal word.of_Z H0).
+           word_Z_unsigned_in H8.
+           rewrite H8 in H7.
+           cbn[Nat.add List.repeat].
+           rewrite repeat_cons.
+           array_app_cons_sep.
+           rewrite repeat_length, <- List.tl_skipn, H17.
+           cbn[List.tl].
+           replace (Z.of_nat (S x5)) with (1 + Z.of_nat x5) by blia. 
+           repeat word_simplify.
+           repeat word_simplify_in H7.
+           change (66) with (Ox "42") in H7.
+           ecancel_assumption. }
+       }
+       split; [blia| auto].
+     }
+     repeat straightline.
+     clear H.
+     array_first_straightline'.
+     clear H3.
+     straightline.
+     split; [auto| split; [auto| ] ].
+     subst P2 P1 Q P.
+
+     unfold message_val, srep_val, cert_val, dele_val, message_ok.
+     unfold size_field, offsets_field, tags_field, tags_offset.
+     cbn[List.length tl map fst snd Array.array Z.of_nat].
+     simpl (Z.of_nat _).
+     unfold fold_left.
+     cbn[fst snd].
+     unfold repeat_dummy.
+     simpl (Z.pos _).
+     repeat word_simplify.
+     ecancel_assumption.
+   Qed.
+     (*
+     remember 
+     
+     refine ((TailRecursion.tailrec (HList.polymorphic_list.cons _ HList.polymorphic_list.nil) ("i"::"buffer"::nil)%list%string (fun V R T M I BUFFER => PrimitivePair.pair.mk (exists i, V = 64 - 4 * (Z.of_nat i) /\ V = word.unsigned I /\ BUFFER = p_addr /\ (array32 (p_addr ^+ (/_ 40)) (List.repeat (word.of_Z (Ox"42")) i) * array32 (p_addr ^+ (/_ (104 - V))) (List.skipn i buf) * array32 p_addr (List.map word.of_Z [5; 64; 64; 164; 316; Z_of_string "SIG"; Z_of_string "PATH"; Z_of_string "SREP"; Z_of_string "CERT"; Z_of_string "INDX"]) * R) M) (fun t m i buff => t = T /\ buff = p_addr /\ (array32 p_addr (List.map word.of_Z ([5; 64; 64; 164; 316; Z_of_string "SIG"; Z_of_string "PATH"; Z_of_string "SREP"; Z_of_string "CERT"; Z_of_string "INDX"] ++ (List.repeat (Ox"42") 16))) * array32 (p_addr ^+ (/_ (104))) (List.skipn 16%nat buf) * R) m))) _ _ _ _ _ _ _);
+      cbn [reconstruct map.putmany_of_list HList.tuple.to_list
+           HList.hlist.foralls HList.tuple.foralls
+           HList.hlist.existss HList.tuple.existss
+           HList.hlist.apply  HList.tuple.apply
+           HList.hlist
+
+           List.repeat Datatypes.length
+           HList.polymorphic_list.repeat HList.polymorphic_list.length
+           PrimitivePair.pair._1 PrimitivePair.pair._2] in *.
+     
+     
+     array_first_straightline'.
+     array_first_straightline'.
+     array_first_before.
+     array_first_after.
+     
+     array_first_straightline'.
+     array_first_after.
+     array_first_before.
+      match goal with
+     | H : ?p ?m |- @WeakestPrecondition.store _ access_size.four ?m ?addr' _ _ =>
+       eapply array_first_store_four_of_sep_32bit;
+       [ reflexivity | ecancel_assumption | try rewrite skipn_length; blia |];
+       repeat straightline
+      end.
+      array_app_cons_sep.
+     match goal with
+     | H : context [array32 (word.add ?a ?b) (List.skipn ?m ?l)] |- _ =>
+       ring_simplify (word.add a b);
+       try (rewrite List.skipn_skipn in H; cbn[Nat.add] in H);
+       array_app_cons_sep
+     end.
+     match goal with
+     | H : ?p ?m |- @WeakestPrecondition.store _ access_size.four ?m ?addr' _ _ =>
+       eapply array_first_store_four_of_sep_32bit;
+       [ reflexivity | ecancel_assumption | try rewrite skipn_length; blia |];
+       repeat straightline
+     end.
+     do 10 array_first_straightline.
+     array_app_cons_sep.
+     array_first_straightline.
+
+     match goal with
+     | H : ?p ?m |- @WeakestPrecondition.store _ Syntax.access_size.four ?m ?addr' _ _ =>
+       match p with
+         context [array32 ?addr ?xs] =>
+         try (rewrite List.skipn_skipn in H; cbn[Nat.add] in H);
+         array_app_cons_sep;
+         try word_simplify_in H;
+         eapply (array_first_store_four_of_sep_32bit _ addr xs _ (word.of_Z 4));
+         [ ecancel_assumption | try rewrite skipn_length; blia |];
+         repeat straightline
+       end
+     end.
+
+     lazymatch goal with
+     | H : ?p ?m |- @WeakestPrecondition.store _ Syntax.access_size.four ?m ?addr' _ _ =>
+       lazymatch p with
+         context [array32 ?addr ?xs] =>
+         subst_words;
+         try (rewrite List.skipn_skipn in H; cbn[Nat.add] in H);
+         array_app_cons_sep;
+         try word_simplify_in H;
+         eapply array_first_store_four_of_sep_32bit;
+         [ reflexivity | ecancel_assumption | try rewrite skipn_length; blia |];
+         repeat straightline
+       end
+     end.
+     eapply (array_first_store_four_of_sep_32bit _ _ _ _ _);
+         [ ecancel_assumption | try rewrite skipn_length; blia |].
+     subst_words.
+     
+     match goal with
+     | H : ?p ?m |- @WeakestPrecondition.store _ Syntax.access_size.four ?m ?addr' _ _ =>
+       match p with
+         context [array32 ?addr ?xs] =>
+         repeat straightline; try (rewrite List.skipn_skipn in H; cbn[Nat.add] in H);
+         array_app_cons_sep;
+         try word_simplify_in H;
+         idtac p
+       end
+     end.
+     
+     
+     array_first_straightline.
+     
+     array_first_straightline.
+     
+     try rewrite List.skipn_skipn in H0.
+     array_app_cons_sep.
+     
+     array_first_straightline.
+     try (rewrite List.skipn_skipn in H2; cbn[Nat.add] in H2).
+     array_app_cons_sep.
+     word_simplify_in H2.
+     array_first_straightline.
+     
+     cbn[Nat.add] in H2.
+     
+     repeat straightline.
+     subst_words.
+     array_app_cons_sep.
+
+     array_first_straightline.
+     match goal with
+     | H : context [List.skipn ?a (List.skipn ?b ?l)] |- _ =>
+       rewrite List.skipn_skipn in H;
+         cbn[Nat.add] in H
+     end.
+     
+     
+     rewrite List.skipn_skipn.
+     change (1 + 1)%nat with 2%nat.
+     repeat straightline.
+     subst_words.
+     array_app_cons_sep.
+     word_simplify_in H2.
+
+     array_first_straightline.
+     repeat straightline.
+     rewrite List.skipn_skipn in H3.
+     array_app_cons_sep.
+     word_simplify_in H3.
+     
+     
+     
+     
+     do 10 (array_straightline; repeat straightline; subst_words).
+
+     refine ((TailRecursion.tailrec (HList.polymorphic_list.cons _ HList.polymorphic_list.nil) ("i"::"buffer"::nil)%list%string (fun V R T M I BUFFER => PrimitivePair.pair.mk (exists i, V = 64 - 4 * (Z.of_nat i) /\ V = word.unsigned I /\ BUFFER = p_addr /\ (array32 (p_addr ^+ (/_ 40)) (List.repeat (word.of_Z (Ox"42")) i) * array32 (p_addr ^+ (/_ (104 - V))) (List.skipn i buf) * array32 p_addr (List.map word.of_Z [5; 64; 64; 164; 316; Z_of_string "SIG"; Z_of_string "PATH"; Z_of_string "SREP"; Z_of_string "CERT"; Z_of_string "INDX"]) * R) M) (fun t m i buff => t = T /\ buff = p_addr /\ (array32 p_addr (List.map word.of_Z ([5; 64; 64; 164; 316; Z_of_string "SIG"; Z_of_string "PATH"; Z_of_string "SREP"; Z_of_string "CERT"; Z_of_string "INDX"] ++ (List.repeat (Ox"42") 16))) * array32 (p_addr ^+ (/_ (104))) (List.skipn 16%nat buf) * R) m))) _ _ _ _ _ _ _);
+      cbn [reconstruct map.putmany_of_list HList.tuple.to_list
+           HList.hlist.foralls HList.tuple.foralls
+           HList.hlist.existss HList.tuple.existss
+           HList.hlist.apply  HList.tuple.apply
+           HList.hlist
+
+           List.repeat Datatypes.length
+           HList.polymorphic_list.repeat HList.polymorphic_list.length
+           PrimitivePair.pair._1 PrimitivePair.pair._2] in *.
+     
+     straightline.
+     
+     match goal with
+     | H : ?p ?m |- @WeakestPrecondition.store _ Syntax.access_size.four ?m ?addr' _ _ => match p with | context [array32 ?addr ?xs] => idtac xs
+                                                                                        end
+     end.
+     match type of H0 with
+     | ((?a * ((?c * ?e) * ?d)) * ?b) ?m => assert (seps [a; b; c; d; e] m)
+     end.
+     { unfold seps; ecancel_assumption. }
+
+     Ltac pick_nat n :=
+       multimatch n with
+       | S ?m => constr:(m)
+       | S ?m => pick_nat m
+       end.
+     
+     try match goal with
+     | H : (seps ?l ?m) |- @WeakestPrecondition.store _ Syntax.access_size.four ?m ?addr' _ _ =>
+       (*remember (Z.to_nat ((\_ (addr' ^- addr)) / 4)) as n eqn:Heqn;
+       ring_simplify (addr' ^- addr) in Heqn;
+       word_Z_unsigned_in Heqn;
+       simpl in Heqn; *)
+
+       (*Make an array lemma with following precondition*)
+       assert (exists i addr ws, nth_error l i = Some (array32 addr ws) /\
+         let n := Z.to_nat (\_(addr' ^- addr) / 4) in (n < List.length ws)%nat);
+         [let L := eval cbv[List.length] in (List.length l) in let r := pick_nat L in exists r; idtac r; fail |]
+       
+       (*eapply (array_store_four_of_sep addr addr' n xs _ (word.of_Z 4))*)
+(* subst ;[try ring | try rewrite List.skipn_length; blia | ecancel_assumption|]*)
+     end.
+     
+     Ltac pick_nat n :=
+       multimatch n with
+       | S ?m => constr:(m)
+       | S ?m => pick_nat m
+       end.
+
+     { (*Pattern to use in array_straightline*)
+       
+       try let r := pick_nat 3%nat in solve[exists r].
+     
+     array_straightline.
+     repeat straightline.
+     clear H0.
+     rewrite firstn_O, app_nil_l in H.
+     array_app_cons_sep.
+     cbn [List.length] in H.
+     word_simplify_in H.
+     rewrite truncate_word_nop_32bit, List.skipn_skipn in H by auto.
+     subst_words.
+     change (1 + 0 + 1)%nat with 2%nat in H.
+     array_straightline.
+     repeat straightline.
+     match goal with
+     | x : context [array32 ?addr ?xs] |- @WeakestPrecondition.store _ Syntax.access_size.four _ ?addr' _ _ =>
+       remember (Z.to_nat ((\_ (addr' ^- addr)) / 4)) as n eqn:Heqn;
+       ring_simplify (addr' ^- addr) in Heqn;
+       word_Z_unsigned_in Heqn;
+       simpl in Heqn;
+       eapply (Scalars.store_array_of_sep addr addr' n xs _ (word.of_Z 4)); subst ;[try ring | try rewrite List.skipn_length; blia | ecancel_assumption|]
+     end.
+     { rewrite List.skipn_length.
+     array_straightline.
+     match goal with
+     | x : context [array32 ?addr ?xs] |- @WeakestPrecondition.store _ Syntax.access_size.four _ ?addr' _ _ =>
+       remember (Z.to_nat ((\_ (addr' ^- addr)) / 4)) as n eqn:Heqn;
+       ring_simplify (addr' ^- addr) in Heqn;
+       word_Z_unsigned_in Heqn;
+       simpl in Heqn;
+       eapply (Scalars.store_array_of_sep addr addr' n xs _ (word.of_Z 4)); subst 
+     end.
+     remember
+     3: { eapply H. eassumption.
+     
+     eapply store_array_of_sep.
+     array_straightline.
+     match goal with
+     | x : context [(array32 ?addr ?xs * ?R) ?m] |- @WeakestPrecondition.store _ Syntax.access_size.four _ ?addr' _ _ =>
+       remember (Z.to_nat ((\_ (addr' ^- addr)) / 4)) as n;
+       ring_simplify (addr' ^- addr) in Heqn;
+       word_Z_unsigned_in Heqn;
+       simpl in Heqn;
+       eapply (Scalars.store_array_of_sep addr addr' n xs _ (word.of_Z 4)); subst ;[try ring | try blia | eassumption|]
+     end.
+     { blia. ring. ring_simplify (p_addr ^- p_addr).
+       
+       ring_simplify (/_ (\_ (/_ 4) * Z.of_nat (Z.to_nat (\_ (/_ 0) / 4)))). simpl.
+       ring. ring_simplify (p_addr ^+ /_ (\_ (/_ 4) * Z.of_nat 0)).
+     array_straightline.
+     { repeat word_simplify.
+       repeat word_Z_unsigned.
+       change (0 / 4) with 0.
+       rewrite Z2Nat.id by blia.
+       ring. }
+       simpl.
+       replace (word.mul (word.of_Z 4) (word.of_Z 0)) with (word.of_Z 0).
+       2: { reflexivity.
+       word_Z_unsigned.
+     { word_simplify.
+      eapply (Scalars.store_array_of_sep p_addr p_addr (Z.to_nat (word.unsigned (word.sub p_addr p_addr) / 4)) buf).
+     match goal with
+     | x : context [(array32 ?addr ?xs * ?R) ?m] |- @WeakestPrecondition.store _ Syntax.access_size.four _ ?addr' _ _ => eapply (Scalars.store_array_of_sep addr addr' (word.divu (word.sub addr' addr) (word.of_Z 4)) xs); [| try ring | try blia |]
+     end.
+     array_straightline.
+     match goal with
+     | x : context [(array32 ?addr ?xs * ?R) ?m] |- @WeakestPrecondition.store _ Syntax.access_size.four _ ?addr' _ _ => eapply (Scalars.store_array_of_sep (word.sub addr' addr) _ _ xs); [| try ring | try blia |]
+     end.
+     array_solve.
+     eapply (store_array_of_sep p_addr _ 0%nat buf _ _);
+       [ring | blia | eassumption |].
+     repeat straightline.
+     rewrite firstn_O, app_nil_l in H0. 
+     array_app_cons_sep.
+     word_simplify_in H0.
+     simpl in H0.
+     eapply (store_array_of_sep p_addr _ 0%nat _ _ (word.of_Z 4));
+       [ring | blia | eassumption |].
+     
+     
      unfold Array.array in H.
      unfold WeakestPrecondition.store.
      
@@ -648,6 +1405,6 @@ Conclusion: Weakestprecondition.store access_size.four m p_addr v post
      simpl.
      word_simplify.
    Admitted.
-   
+   *)
 End WithParameters.
 
